Sodium.lean
@@ -1,1 +1,9 @@
 import «Sodium».Crypto.Monad
+import «Sodium».Data.Digest
+
+open Lean Sodium Crypto
+
+#eval show MetaM Json from CryptoM.toMetaM fun _ => do
+  let sig ← sign (json% {some: "string"})
+  println! digest sig
+  return encode sig
