Sodium/Crypto/Types.lean
@@ -1,4 +1,4 @@
-import Sodium.Data.Encodable.Basic
+import Sodium.Data.Encodable.WType
 import Sodium.Crypto.Spec
 
 open Lean
@@ -76,7 +76,6 @@ abbrev Nonce (spec : Spec) [spec.HasValidShape `nonce] :=
   ByteVector spec[`nonce]
 
 structure NonceId (spec : Spec) where
-  Δh : spec.HasValidShape `nonce
   get : (h : spec.HasValidShape `nonce) → Nonce spec
 
 abbrev Salt (τ : Sodium σ) (spec : Spec) [h : spec.HasValidShape `salt] :=
@@ -92,7 +91,6 @@ abbrev PublicKey (spec : Spec) [spec.HasValidShape `publickey] :=
   ByteVector spec[`publickey]
 
 structure PublicKeyId (spec : Spec) where
-  Δh : spec.HasValidShape `publickey
   get : (h : spec.HasValidShape `publickey) → PublicKey spec
 
 abbrev SharedKey (τ : Sodium σ) (spec : Spec) [h : spec.HasValidShape `sharedkey] :=
@@ -110,28 +108,24 @@ abbrev Hash (spec : Spec) [spec.HasValidShape `hash] :=
   ByteVector spec[`hash]
 
 structure HashId (spec : Spec) where
-  Δh : spec.HasValidShape `hash
   get : (h : spec.HasValidShape `hash) → Hash spec
 
 abbrev Context (spec : Spec) [spec.HasValidShape `context] :=
   ByteVector spec[`context]
 
 structure ContextId (spec : Spec) where
-  Δh : spec.HasValidShape `context
   get : (h : spec.HasValidShape `context) → Context spec
 
 abbrev Header (spec : Spec) [spec.HasValidShape `header] :=
   ByteVector spec[`header]
 
 structure HeaderId (spec : Spec) where
-  Δh : spec.HasValidShape `header
   get : (h : spec.HasValidShape `header) → Header spec
 
 abbrev Signature (spec : Spec) [spec.HasValidShape `signature] :=
   ByteVector spec[`signature]
 
 structure SignatureId (spec : Spec) where
-  Δh : spec.HasValidShape `signature
   get : (h : spec.HasValidShape `signature) → Signature spec
 
 structure SignedJson (spec : Spec) [spec.HasValidShape `signature] [spec.HasValidShape `publickey] where
@@ -141,7 +135,6 @@ structure SignedJson (spec : Spec) [spec.HasValidShape `signature] [spec.HasVali
   deriving ToJson, FromJson
 
 structure SignedJsonId (spec : Spec) where
-  Δh : spec.HasValidShape `signature ∧ spec.HasValidShape `publickey
   get : (h_sig : spec.HasValidShape `signature) → (h_key : spec.HasValidShape `publickey) → SignedJson spec
 
 namespace SignedJson
